prove inv_func_copy_out_sound

core/ConcreteHoare.v
@@ -30,12 +30,6 @@ Context `{@Target tags_t Expression}.
 
 Variable ge : (@genv tags_t _).
 
-(* shallow assertions *)
-Definition assertion := state -> Prop.
-Definition arg_assertion := list Sval -> state -> Prop.
-Definition ret_assertion := Val -> state -> Prop.
-Definition arg_ret_assertion := list Sval -> Val -> state -> Prop.
-
 Lemma hoare_stmt_assign' : forall p a_mem a_ext tags lhs rhs typ a_mem' ret_post lv sv,
   is_call_expression rhs = false ->
   is_no_dup (map fst a_mem) ->
@@ -52,5 +46,249 @@ Proof.
   - apply hoare_expr_det_intro, eval_expr_sound; eassumption.
   - apply eval_write_sound; only 1 : apply is_no_dup_NoDup; eassumption.
 Qed.
+
+(* Inductive Disjoint {A} : list A -> list A -> Prop :=
+  | Disjoint_nil : forall al', Disjoint  [] al'
+  | Disjoint_cons : forall a al al', ~In a al' -> Disjoint al al' -> Disjoint (a :: al) al'.
+
+Fixpoint is_disjoint (al bl : list path) : bool :=
+  match al with
+  | x :: al => ~~(is_in x bl) && is_disjoint al bl
+  | [] => true
+  end.
+
+Lemma is_disjoint_Disjoint : forall (al bl : list path),
+  is_disjoint al bl -> Disjoint al bl.
+Proof.
+  induction al; intros.
+  - constructor.
+  - simpl in H0. rewrite Reflect.andE in H0. destruct H0.
+    constructor.
+    + apply not_is_in_not_In; auto.
+    + auto.
+Qed. *)
+
+Definition ret_implies (P Q : Hoare.ret_assertion) :=
+  forall retv st, P retv st -> Q retv st.
+
+Definition ret_exists {A} (a : A -> Hoare.ret_assertion) : Hoare.ret_assertion :=
+  fun retv st => ex (fun x => a x retv st).
+
+Definition arg_ret_exists {A} (a : A -> Hoare.arg_ret_assertion) : Hoare.arg_ret_assertion :=
+  fun args retv st => ex (fun x => a x args retv st).
+
+Declare Scope post_cond.
+Delimit Scope post_cond with post_cond.
+Notation "'EX' x .. y , P " :=
+  (arg_ret_exists (fun x => .. (arg_ret_exists (fun y => P%post_cond)) ..)) (at level 65, x binder, y binder, right associativity) : post_cond.
+
+Inductive inv_func_copy_out (out_params : list path) : Hoare.ret_assertion -> Hoare.arg_ret_assertion -> Prop :=
+  | inv_func_copy_out_base : forall a_arg a_ret a_mem a_ext,
+      length out_params = length a_arg ->
+      NoDup (out_params ++ (map fst a_mem)) ->
+      inv_func_copy_out out_params
+        (RET a_ret (MEM (eval_write_vars a_mem out_params a_arg) (EXT a_ext)))
+        (ARG_RET a_arg a_ret (MEM a_mem (EXT a_ext)))
+  | inv_func_copy_out_ex : forall {A} (P : A -> Hoare.ret_assertion) Q,
+      (forall (x : A), inv_func_copy_out out_params (P x) (Q x)) ->
+      inv_func_copy_out out_params (ret_exists P) (arg_ret_exists Q).
+
+Axiom AList_get_set_some_neq : forall (a_mem : mem_assertion) (p p' : path) sv,
+  p <> p' ->
+  AList.get (AList.set_some a_mem p' sv) p = AList.get a_mem p.
+
+Lemma eval_read_var_eval_write_vars_disjoint : forall p ps vs a_mem,
+  ~In p ps ->
+  eval_read_var (eval_write_vars a_mem ps vs) p = eval_read_var a_mem p.
+Proof.
+  induction ps; intros.
+  - auto.
+  - destruct vs. { auto. }
+    change (eval_write_vars a_mem (a :: ps) (v :: vs)) with
+      (eval_write_vars (eval_write_var a_mem a v) ps vs).
+    rewrite IHps. 2 : { intro. apply H0. right. auto. }
+    apply AList_get_set_some_neq.
+    intro. subst. apply H0. left. auto.
+Qed.
+
+Lemma eval_write_vars_cons : forall p ps v vs a_mem,
+  eval_write_vars a_mem (p :: ps) (v :: vs) = eval_write_vars (eval_write_var a_mem p v) ps vs.
+Proof.
+  reflexivity.
+Qed.
+
+Lemma eval_read_var_eval_write_var : forall a_mem p v,
+  eval_read_var (eval_write_var a_mem p v) p = Some v.
+Proof.
+  intros. eapply AList.set_some_get.
+Qed.
+
+Lemma eval_read_vars_eval_write_vars : forall out_params a_arg a_mem,
+  length out_params = length a_arg ->
+  NoDup out_params ->
+  eval_read_vars (eval_write_vars a_mem out_params a_arg) out_params = map Some a_arg.
+Proof.
+  induction out_params; intros.
+  - destruct a_arg; only 2 : inv H0.
+    auto.
+  - destruct a_arg; only 1 : inv H0.
+    simpl. f_equal.
+    + rewrite eval_write_vars_cons.
+      rewrite eval_read_var_eval_write_vars_disjoint.
+      * apply eval_read_var_eval_write_var.
+      * inv H1. auto.
+    + change (eval_write_vars a_mem (a :: out_params) (v :: a_arg)) with
+        (eval_write_vars (eval_write_var a_mem a v) out_params a_arg).
+      apply IHout_params.
+      * auto.
+      * inv H1. auto.
+Qed.
+
+Lemma lift_option_inv : forall {A} (xl : list (option A)) (al : list A),
+  lift_option xl = Some al ->
+  xl = map Some al.
+Proof.
+  induction xl; intros.
+  - inv H0. auto.
+  - destruct a.
+    + simpl in H0. destruct (lift_option xl).
+      * inv H0. simpl; f_equal; auto.
+      * inv H0.
+    + inv H0.
+Qed.
+
+Lemma eval_write_var_disjoint : forall a_mem p sv,
+  ~In p (map fst a_mem) ->
+  eval_write_var a_mem p sv = a_mem ++ [(p, sv)].
+Proof.
+  induction a_mem; intros.
+  - auto.
+  - simpl. destruct a as [p' sv'].
+    destruct (EquivDec.list_eqdec EquivUtil.StringEqDec p p') as [H_eqb | H_eqb].
+    + cbv in H_eqb. subst. exfalso. apply H0. constructor. auto.
+    + rewrite IHa_mem; auto.
+      intro. apply H0. right. apply H1.
+Qed.
+
+Lemma eval_write_vars_disjoint' : forall a_mem pvs,
+  NoDup (map fst pvs ++ map fst a_mem) ->
+  fold_left (fun a '(p, sv) => eval_write_var a p sv) pvs a_mem = a_mem ++ pvs.
+Proof.
+  intros a_mem pvs; revert a_mem.
+  induction pvs; intros.
+  - simpl. rewrite app_nil_r. auto.
+  - simpl.
+    destruct a as [p sv].
+    rewrite eval_write_var_disjoint. 2 : {
+      inv H0.
+      intro. apply H3. apply in_app_iff. auto.
+    }
+    rewrite IHpvs.
+    + rewrite <- app_assoc. auto.
+    + (* some stupid NoDup proof *)
+      eapply Permutation.Permutation_NoDup. 2 : { apply H0. }
+      apply Permutation.Permutation_trans with ((map fst pvs ++ [p]) ++ map fst a_mem).
+      { apply Permutation.Permutation_app.
+        - apply Permutation.Permutation_cons_append.
+        - apply Permutation.Permutation_refl.
+      }
+      rewrite <- app_assoc.
+      apply Permutation.Permutation_app.
+      * apply Permutation.Permutation_refl.
+      * rewrite map_app. apply Permutation.Permutation_cons_append.
+Qed.
+
+Lemma eval_write_vars_disjoint : forall a_mem ps svs,
+  length ps = length svs ->
+  NoDup (ps ++ (map fst a_mem)) ->
+  eval_write_vars a_mem ps svs = a_mem ++ (combine ps svs).
+Proof.
+  unfold eval_write_vars.
+  intros. apply eval_write_vars_disjoint'.
+  rewrite Utils.map_fst_combine; auto.
+Qed.
+
+Lemma eval_write_vars_implies' : forall a_mem out_params a_arg,
+  length out_params = length a_arg ->
+  NoDup (out_params ++ (map fst a_mem)) ->
+  forall m,
+    mem_denote (eval_write_vars a_mem out_params a_arg) m ->
+    mem_denote a_mem m.
+Proof.
+  intros. rewrite eval_write_vars_disjoint in H2; auto.
+  clear H0 H1.
+  induction a_mem; intros.
+  - constructor.
+  - constructor.
+    + apply H2.
+    + apply IHa_mem, H2.
+Qed.
+
+Lemma eval_write_vars_implies : forall a_mem out_params a_arg a_ext,
+  length out_params = length a_arg ->
+  NoDup (out_params ++ (map fst a_mem)) ->
+  implies
+    (MEM (eval_write_vars a_mem out_params a_arg) (EXT a_ext))
+    (MEM a_mem (EXT a_ext)).
+Proof.
+  unfold implies; intros.
+  destruct st; destruct H2; split.
+  - eapply eval_write_vars_implies'; eauto.
+  - auto.
+Qed.
+
+Lemma NoDup_app_remove_2 : forall {A} (l l' : list A),
+  NoDup (l ++ l') ->
+  NoDup l.
+Proof.
+  intros. induction l.
+  - constructor.
+  - inv H0.
+    constructor.
+    + rewrite in_app_iff in H3. auto.
+    + auto.
+Qed.
+
+Lemma inv_func_copy_out_sound_part1 : forall params a_arg a_ret a_mem a_ext,
+  length (filter_out params) = length a_arg ->
+  NoDup ((filter_out params) ++ (map fst a_mem)) ->
+  hoare_func_copy_out
+    (RET a_ret (MEM (eval_write_vars a_mem (filter_out params) a_arg) (EXT a_ext))) params
+    (ARG_RET a_arg a_ret (MEM a_mem (EXT a_ext))).
+Proof.
+  unfold hoare_func_copy_out; intros.
+  epose proof (eval_read_vars_eval_write_vars (filter_out params) _ _ H0 (NoDup_app_remove_2 _ _ H1)).
+  unfold extract_parameters in H3.
+  apply lift_option_inv in H3.
+  pose proof (eval_read_vars_sound _ _ _ _ H4 _ _ (proj2 H2) H3).
+  split. { auto. }
+  split. { apply H2. }
+  eapply eval_write_vars_implies; eauto.
+  apply H2.
+Qed.
+
+Lemma inv_func_copy_out_sound : forall params P Q,
+  inv_func_copy_out (filter_out params) P Q ->
+  hoare_func_copy_out P params Q.
+Proof.
+  intros.
+  induction H0.
+  - apply inv_func_copy_out_sound_part1; auto.
+  - unfold hoare_func_copy_out. intros.
+    destruct H2 as [x ?].
+    exists x.
+    apply H1; eauto.
+Qed.
+
+Lemma hoare_func_internal' : forall p pre_arg pre_mem pre_ext params init body targs mid1_mem mid2 mid3 post,
+  length (filter_in params) = length pre_arg ->
+  is_no_dup (map fst pre_mem) ->
+  eval_write_vars pre_mem (filter_in params) pre_arg = mid1_mem ->
+  hoare_block ge p (MEM mid1_mem (EXT pre_ext)) init (mk_post_assertion mid2 mid3) ->
+  hoare_block ge p mid2 body (return_post_assertion_1 mid3) ->
+  inv_func_copy_out (filter_out params) mid3 post ->
+  hoare_func ge p (ARG pre_arg (MEM pre_mem (EXT pre_ext))) (FInternal params init body) targs post.
+Proof.
+Admitted.
 
 End ConcreteHoare.
